Introduce the run and the derivation

src/TemporalLogic.v
@@ -17,29 +17,25 @@ Section TEMPORAL_LOGIC.
   Notation "p .? a" := (prop p a) (at level 51).
 
   Inductive TL: Type :=
-  | loop (gold: TL)
-         (current: TL)
+  | true
+    : TL
+  | false
+    : TL
+  | globally (prop: Instant)
+    : TL
+  | eventually (prop: Instant)
     : TL
   | next (tl: TL)
     : TL
   | switch (tl1: TL)
            (prop: Instant)
            (tl2: TL)
-    : TL
-  | globally (prop: Instant)
-    : TL
-  | eventually (prop: Instant)
-    : TL
-  | true
-    : TL
-  | false
     : TL.
 
   Fixpoint halt_satisfies
              (tl: TL)
     : Prop :=
     match tl with
-    | loop _ current => halt_satisfies current
     | eventually _ => False
     | next _ => False
     | switch before _ _ => halt_satisfies before
@@ -51,7 +47,6 @@ Section TEMPORAL_LOGIC.
     : {halt_satisfies tl}+{~halt_satisfies tl}.
     refine (
         match tl with
-        | loop _ current => decide_dec (halt_satisfies_dec current)
         | eventually _ => false_dec
         | next _ => false_dec
         | switch before _ _ => decide_dec (halt_satisfies_dec before)
@@ -61,23 +56,54 @@ Section TEMPORAL_LOGIC.
       firstorder.
     Defined.
 
+  Inductive TL_step
+    : TL -> TL -> Prop :=
+  | true_stays_true: TL_step true true
+  | false_stays_false: TL_step false false
+  | globally_stays_globally
+      (prop: Instant)
+    : TL_step (globally prop) (globally prop)
+  | globally_can_fail
+      (prop: Instant)
+    : TL_step (globally prop) false
+  | eventually_stays_eventually
+      (prop: Instant)
+    : TL_step (eventually prop) (eventually prop)
+  | eventually_can_succeed
+      (prop: Instant)
+    : TL_step (eventually prop) true
+  | next_steps_unwrap
+      (tl: TL)
+    : TL_step (next tl) tl
+  | switch_steps_before
+      (tl1 tl2 tl3: TL)
+      (prop: Instant)
+      (Hderive: TL_step tl1 tl2)
+    : TL_step (switch tl1 prop tl3) (switch tl2 prop tl3)
+  | switch_step_after_small
+      (tl1 tl2: TL)
+      (prop: Instant)
+    : TL_step (switch tl1 prop tl2) tl2
+  | switch_can_fail
+      (tl1 tl2: TL)
+      (prop: Instant)
+    : TL_step (switch tl1 prop tl2) false.
+
   Fixpoint instruction_satisfies
            (a: A)
            (tl: TL)
     : Prop :=
     match tl with
-    | loop _ current
-      => instruction_satisfies a current
+    | true => True
+    | false => False
+    | globally prop => prop.? a
+    | eventually tl => True
     | next _
       => True
     | switch before prop after
       => (prop.? a -> instruction_satisfies a after
                       /\ halt_satisfies before)
          /\ (~prop.? a -> instruction_satisfies a before)
-    | globally prop => prop.? a
-    | eventually tl => True
-    | true => True
-    | false => False
     end.
 
   Fixpoint instruction_satisfies_dec
@@ -86,26 +112,25 @@ Section TEMPORAL_LOGIC.
     : {instruction_satisfies a tl}+{~instruction_satisfies a tl}.
     refine (
         match tl with
-        | loop _ current
-          => decide_dec (instruction_satisfies_dec a current)
-        | next _
+        | true
           => true_dec
+        | false
+          => false_dec
         | globally prop
           => decide_dec (prop? a)
+        | eventually prop
+          => true_dec
+        | next _
+          => true_dec
         | switch before p after
           => if p? a
              then decide_dec (sumbool_and _ _ _ _
                                           (instruction_satisfies_dec a after)
                                           (halt_satisfies_dec before))
              else decide_dec (instruction_satisfies_dec a before)
-        | eventually prop
-          => true_dec
-        | true
-          => true_dec
-        | false
-          => false_dec
         end
       ); cbn; trivial.
+    + intro False; destruct False.
     + split.
       ++ intro _H; exact a0.
       ++ intro False; apply False in p0; destruct p0.
@@ -123,7 +148,6 @@ Section TEMPORAL_LOGIC.
       apply False in n.
       apply n0 in n.
       destruct n.
-    + intro False; destruct False.
   Defined.
 
   Fixpoint tl_step
@@ -132,18 +156,12 @@ Section TEMPORAL_LOGIC.
     : TL :=
     if instruction_satisfies_dec a tl
     then match tl with
-         | loop gold current
-           => match (tl_step a current) with
-              | true => loop gold gold
-              | false => false
-              | c' => loop gold c'
-              end
          | next tl
            => tl
          | switch before p after
            => if p? a
               then after
-              else switch before p after
+              else switch (tl_step a before) p after
          | eventually p
            => if p ? a
               then true
@@ -152,7 +170,44 @@ Section TEMPORAL_LOGIC.
            => x
          end
     else false.
+
+  Lemma TL_step_is_tl_step
+    : forall (a: A)
+             (tl: TL),
+      TL_step tl (tl_step a tl).
+  Proof.
+    induction tl.
+    + constructor.
+    + constructor.
+    + cbn; destruct (prop0 ? a); constructor.
+    + cbn; destruct (prop0 ? a); constructor.
+    + cbn; constructor.
+    + cbn.
+      destruct (prop0 ? a).
+      ++ destruct (instruction_satisfies_dec a tl2);
+           destruct (halt_satisfies_dec tl1);
+           cbn.
+         +++ constructor.
+         +++ constructor.
+         +++ constructor.
+         +++ constructor.
+      ++ destruct (instruction_satisfies_dec a tl1).
+         +++ constructor.
+             exact IHtl1.
+         +++ constructor.
+  Qed.
+
 End TEMPORAL_LOGIC.
+
+Arguments true [_].
+Arguments false [_].
+Arguments next [_].
+Arguments globally [_].
+Arguments eventually [_].
+Arguments switch [_].
+
+Arguments TL_step [_].
+Arguments tl_step [_].
 
 Section RUN_TL.
   Variable (I: Type -> Type).
@@ -172,11 +227,240 @@ Section RUN_TL.
     | ret a => (a, int, tl)
     | instr i => (evalInstruction i int,
                     execInstruction i int,
-                    tl_step _ (instruction i) tl)
+                    tl_step (instruction i) tl)
     | bind p' f => runTL (snd (fst (runTL int p' tl)))
-                           (f (fst (fst (runTL int p' tl))))
-                           (snd (runTL int p' tl))
+                         (f (fst (fst (runTL int p' tl))))
+                         (snd (runTL int p' tl))
     end.
+
+  Inductive TL_run
+            {A: Type}
+    : TL A -> TL A -> Prop :=
+  | tl_run_refl
+      (tl: TL A)
+    : TL_run tl tl
+  | tl_run_small_step
+      (from to: TL A)
+      (Hstep: TL_step from to)
+    : TL_run from to
+  | tl_run_big_step
+      (from tl to: TL A)
+      (Hstep: TL_step from tl)
+      (Hrun: TL_run tl to)
+    : TL_run from to.
+
+  Lemma tl_step_run_trans
+        {A: Type}
+        (tl tl' tl'': TL A)
+    : TL_step tl tl'
+      -> TL_step tl' tl''
+      -> TL_run tl tl''.
+  Proof.
+    intros H1 H2.
+    apply (tl_run_big_step tl tl' tl'').
+    + exact H1.
+    + apply (tl_run_small_step tl' tl'' H2).
+  Qed.
+
+  Lemma tl_run_step_run
+        {A: Type}
+        (tl tl' tl'': TL A)
+    : TL_run tl tl'
+      -> TL_step tl' tl''
+      -> TL_run tl tl''.
+  Proof.
+    intros H1 H2.
+    induction H1.
+    ++ constructor.
+       exact H2.
+    ++ apply (tl_step_run_trans from to tl'' Hstep H2).
+    ++ apply IHTL_run in H2.
+       apply (tl_run_big_step from tl tl'' Hstep H2).
+  Qed.
+
+  Lemma tl_run_trans
+        {A: Type}
+        (tl tl' tl'': TL A)
+    : TL_run tl tl'
+      -> TL_run tl' tl''
+      -> TL_run tl tl''.
+  Proof.
+    intros H1 H2.
+    induction H1.
+    + exact H2.
+    + apply (tl_run_big_step from to tl'' Hstep H2).
+    + apply IHTL_run in H2.
+      apply (tl_run_big_step from tl tl'' Hstep H2).
+  Qed.
+
+  Lemma next_derives_big
+        {A: Type}
+        (tl tl': TL A)
+        (Hderive: TL_run tl tl')
+    : TL_run (next tl) tl'.
+  Proof.
+    assert (TL_run (next tl) tl)
+      as Hbefore
+        by (repeat constructor).
+    apply (tl_run_trans (next tl) tl tl' Hbefore Hderive).
+    Qed.
+
+  Lemma switch_derives_after_big
+        (tl1 tl2 tl3: TL ISet)
+        (prop: Instant ISet)
+        (Hderive: TL_run tl2 tl3)
+    : TL_run (switch tl1 prop tl2) tl3.
+  Proof.
+    assert (TL_run (switch tl1 prop tl2) tl2)
+      as Hrun'
+        by (repeat constructor).
+    apply (tl_run_trans (switch tl1 prop tl2) tl2 tl3 Hrun' Hderive).
+  Qed.
+
+  Lemma switch_derives_before_big
+        (tl1 tl2 tl3: TL ISet)
+        (prop: Instant ISet)
+        (Hderive: TL_run tl1 tl2)
+    : TL_run (switch tl1 prop tl3) (switch tl2 prop tl3).
+  Proof.
+    induction Hderive.
+    + apply tl_run_refl.
+    + apply tl_run_small_step.
+      constructor.
+      exact Hstep.
+    + apply (tl_run_trans (switch from prop tl3) (switch tl prop tl3)).
+      ++ repeat constructor.
+         exact Hstep.
+      ++ exact IHHderive.
+  Qed.
+
+  Lemma TL_run_is_runTL
+    : forall {A: Type}
+             (p: Program I A)
+             (tl: TL ISet)
+             (int: Interp I),
+      TL_run tl (snd (runTL int p tl)).
+  Proof.
+    induction p.
+    + intros tl int.
+      cbn.
+      apply (tl_run_trans tl
+                          (snd (runTL int p tl))
+                          (snd
+                             (runTL (snd (fst (runTL int p tl))) (f (fst (fst (runTL int p tl))))
+                                    (snd (runTL int p tl))))).
+      ++ apply IHp.
+      ++ apply H.
+    + intros tl int.
+      cbn.
+      constructor.
+      apply TL_step_is_tl_step.
+    + intros tl int.
+      cbn.
+      apply tl_run_refl.
+  Qed.
+
+  Inductive TL_derive
+            {A: Type}
+    : TL A -> TL A -> Prop :=
+  | tl_derives_tl
+      (x: TL A)
+    : TL_derive x x
+  | true_derives_true
+    : TL_derive true true
+  | false_derives_false
+    : TL_derive false false
+  | globally_derives_globally
+      (prop: Instant A)
+    : TL_derive (globally prop) (globally prop)
+  | globally_derives_fail
+      (prop: Instant A)
+    : TL_derive (globally prop) false
+  | eventually_derives_eventually
+      (prop: Instant A)
+    : TL_derive (eventually prop) (eventually prop)
+  | eventually_derives_fail
+      (prop: Instant A)
+    : TL_derive (eventually prop) true
+  | next_derives_unwrap
+      (tl tl': TL A)
+      (Hderive: TL_derive tl tl')
+    : TL_derive (next tl) tl'
+  | switch_derives_before
+      (before after tl: TL A)
+      (prop: Instant A)
+      (Hderive: TL_derive before tl)
+    : TL_derive (switch before prop after) (switch tl prop after)
+  | switch_derives_after
+      (before after tl: TL A)
+      (prop: Instant A)
+      (Hderive: TL_derive after tl)
+    : TL_derive (switch before prop after) tl
+  | switch_derives_fail
+      (before after: TL A)
+      (prop: Instant A)
+    : TL_derive (switch before prop after) false.
+
+  Lemma tl_step_is_tl_derive
+        {A: Type}
+    : forall (tl tl': TL A),
+      TL_step  tl tl' -> TL_derive tl tl'.
+  Proof.
+    induction tl; intros; inversion H; subst.
+    + constructor.
+    + constructor.
+    + constructor.
+    + constructor.
+    + constructor.
+    + constructor.
+    + constructor; constructor.
+    + constructor.
+      apply IHtl1.
+      exact Hderive.
+    + constructor; constructor.
+    + apply switch_derives_fail.
+  Qed.
+
+  Lemma tl_run_switch_before
+        {A: Type}
+  : forall (tl tl' tl2: TL A)
+           (prop: Instant A),
+      TL_run tl tl'
+      -> TL_run (switch tl prop tl2) (switch tl' prop tl2).
+  Proof.
+    induction tl.
+    + intros.
+      assert (tl' = true) as Heqt.
+  Admitted.
+
+  Lemma tl_run_implies_tl_derive
+        {A: Type}
+    : forall (tl tl': TL A),
+      TL_derive tl tl' -> TL_run  tl tl'.
+  Proof.
+    induction tl.
+    + intros tl' Hderive.
+      inversion Hderive; subst; constructor.
+    + intros tl' Hderive.
+      inversion Hderive; subst; constructor.
+    + intros tl' Hderive.
+      inversion Hderive; subst; repeat constructor.
+    + intros tl' Hderive.
+      inversion Hderive; subst; repeat constructor.
+    + intros tl' Hderive.
+      inversion Hderive; subst.
+      ++ apply tl_run_refl.
+      ++ assert (TL_run (next tl) tl)
+          as Hstep
+            by (repeat constructor).
+         apply (tl_run_trans (next tl) tl tl' Hstep).
+         apply IHtl.
+         apply Hderive0.
+    + intros tl' Hderive.
+      inversion Hderive; subst.
+      ++ apply tl_run_refl.
+      ++
+  Admitted.
 
   Lemma run_tl_run_program_interp_eq
         {A: Type}
